<section xmlns:xi="http://www.w3.org/2001/XInclude"><title> Solutions Types </title>

	<p>
		We have just discussed some important ideas that will aid us in understanding what it means to be a solution to an differential equation. You will see that the next two statement are practically identical (except the blue terms).
	</p>

	<ul>
		<li>
			<m>\color{blue}{x}</m> (a <m>\color{blue}{\text{number}}</m>) is a solution to an <m>\color{blue}{\text{algebraic}}</m> equation if we get the same result on the left and right-hand side of the equation after substituting <m>\color{blue}{x}</m> into the entire equation.
		</li>
		<li>
			<m>\color{blue}{y}</m> (a <m>\color{blue}{\text{function}}</m>) is a solution to a <m>\color{blue}{\text{differential}}</m> equation if we get the same result on the left and right-hand side of the equation after substituting <m>\color{blue}{y}</m> into the entire equation.
		</li>
	</ul>
	
	<!--
	<p>
		Recall, <m>\color{blue}{x}</m> (a <m>\color{blue}{\text{number}}</m>) is a solution to an <m>\color{blue}{\text{algebraic}}</m>	equation if:
		<sidebyside widths="90%" margins="auto" valign="middle">
		<p>
			If we get the same result on the left and right-hand side of the equation after plugging <m>\color{blue}{x}</m> into the entire equation, then we say <m>\color{blue}{x}</m> is a solution to the <m>\color{blue}{\text{algebraic}}</m> equation.
		</p>
		</sidebyside>
	</p>
	<p>
		Similarly, <m>\color{blue}{y}</m> (a <m>\color{blue}{\text{function}}</m>) is a solution to an <m>\color{blue}{\text{differential}}</m> equation if:
		<sidebyside widths="90%" margins="auto" valign="middle">
		<p>
			If we get the same result on the left and right-hand side of the equation after plugging <m>\color{blue}{y}</m> into the entire equation, then we say <m>\color{blue}{y}</m> is a solution to the <m>\color{blue}{\text{differential}}</m> equation.
		</p>
		</sidebyside>
	</p>
	-->
	

	<p>
	In all of the previous examples, we verified that one particular function was a solution to the DE, but as previously mentioned, we know that there may be more. It turns out, differential equations generally have infinitely many solutions. We can use <xref ref="example-de-solution-05" /> to illustrate this.
	</p>

	<p>
	In this example, we showed that the function <m>y = c_1e^{-3t} + c_2e^{4t}</m> was a solution <m>y'' - y' - 12y = 0</m>.
	</p>

	<p>
	Notice that we were able to verify the solution, even though the constants, <m>c_1</m> and <m>c_2</m>, were not known. This suggests that you can substitute any values of <m>c_1</m> and <m>c_2</m> into the solution and it will still be a solution to the DE. <em> Try it! </em>
	</p>

	<p>
	Now, since there are infinitely many choices for <m>c_1</m> and <m>c_2</m>,	then, logically, there must be infinitely many solutions to the DE,	<m>y'' - y' - 12y = 0</m>.
	</p>

	<definition xml:id="def-general-solution">
	<statement>
		Given a differential equation, the collection of all solutions of this DE is called the <term>family of solutions</term> of this DE. The form of these solutions is called the <term>general solution</term> of this DE. A single solution from the family of solutions is called a <term>particular solution</term>.
	</statement>
	</definition>

	<remark xml:id="remark-general-solution-01">
	<p>
		A <em>family of solutions</em> can be viewed as the collection of all <em>particular solutions</em>. Conversely, a <em>particular solution</em> can be viewed as a member of the <em>family of solutions</em>.
	</p>
	</remark>

	<p>
	In the context of <xref ref="example-de-solution-05" />, all of the following would be true:
	<ul>
		<li> 	<m>y = c_1e^{-3t} + c_2e^{4t}</m> is the solution to
		<m>y'' - y' - 12y = 0</m>. </li>
		<li> 	<m>y = c_1e^{-3t} + c_2e^{4t}</m> is the <term>general solution</term>
		to the <m>y'' - y' - 12y = 0</m>. </li>
		<li> 	Any solution that has the form: <m>y = c_1e^{-3t} + c_2e^{4t}</m> is in the <term>family of solutions</term> for
		<m>y'' - y' - 12y = 0</m>. </li>
		<li> 	<m>y = -e^{-3t} + 7e^{4t}</m> is a <term>particular solution</term> to
		<m>y'' - y' - 12y = 0 \,\,</m> (<m>c_1 = -1</m>, <m>c_2 = 7</m>).</li>
		<li> 	<m>y = -e^{-3t} + 7e^{4t}</m> is in the <term>family of solutions</term> for <m>y'' - y' - 12y = 0</m> since it has the form:
		<m>y = c_1e^{-3t} + c_2e^{4t}</m> where <m>c_1 = -1</m> and
		<m>c_2 = 7</m>.</li>
	</ul>
	</p>

	<remark xml:id="remark-general-solution-02">
	<p>
		When working on your own problems, remember that the following three statements are referring to the exact same thing.
		<ul>
		<li> Solve the following DE. </li>
		<li> Find the <em>general solution</em> to the following DE. </li>
		<li> Find the <em>family of solutions</em> for the following DE. </li>
		</ul>
	</p>
	</remark>

	<p>
	We spend a lot of time solving equations, but do you even remember what it means to be
	a solution? Let's review what it means to be a solution to an algebraic equation 
	(as in question <xref ref="alg_eqn_soln"/>), and then what it means to be a solution to a differential equation (as in question <xref ref="diff_eqn_soln"/>), and then we'll extend those ideas in questions <xref ref="soln_form1"/> and <xref ref="soln_form2"/>.

	<ol>
	<li>
	<p>
	Verify that <m>x = 3</m> is a solution to the equation 
	
	<men xml:id="alg_eqn_soln">2x^2 + 3 = 7x.</men>
	
	</p>
	
	<p>
	What confirms that <m>x = 3</m> is a solution? 
	<answer>
		the LHS = RHS after substituting <m>x = 3</m> into both sides of the equation.
	</answer>	
	</p>
	
	<p>	
	(<em> Note: Do not rearrange the equation to solve for <m>x</m>. That would be the
	process of finding a solution; you are asked to verify a solution.</em>)
	</p>	
	<p/>
	<solution>
	We substitute <m>x = 3</m> into the left hand side (LHS) of the equation, 
	and then into the right hand side (RHS) of the equation:
	
	<md>
		<mrow>\text{LHS}	\amp= 2x^2 + 3										</mrow>
		<mrow>				\amp= 2(3)^2 + 3									</mrow>
		<mrow>				\amp= 18 + 3										</mrow>
		<mrow>				\amp= 21											</mrow>
		<mrow>				\amp 												</mrow>
		<mrow>\text{RHS}	\amp= 7x											</mrow>
		<mrow>				\amp= 7(3)											</mrow>
		<mrow>				\amp= 21											</mrow>	
	</md>
	
	Since we get the same result when we substitute the solution into the RHS and 
	into the LHS, we have confirmed that <m>x = 3</m> is a solution to the equation.
	</solution>
	<!-- Is this answer necessary?
	<answer>
		Since we get the same result (21) when we substitute the solution into the 
		RHS and into the LHS, we confirm that <m>x = 3</m> is a solution to the equation.
	</answer>
	-->
	
	</li>

	<li>
	<p>
	Verify that <m>y = c_1 \sin x + c_2 \cos x</m> is a solution to the DE 
	
	<men xml:id="diff_eqn_soln">\DS \frac{d^2y}{dx^2} + y = 0.</men>
	
	</p>
	
	<hint>
	Look back at the previous question and think about what it means to be a solution 
	to a DE.
	</hint>
	<solution>
	We need to substitute into the DE. In order to substitute into the left hand side, 
	we need to know the second derivative. So we begin by finding that.
	
	<md>
		<mrow>						y	\amp= c_1 \sin x + c_2 \cos x			</mrow>
		<mrow>	\Rightarrow \quad   y'	\amp= c_1 \cos x - c_2 \sin x			</mrow>
		<mrow>	\Rightarrow \quad   y''	\amp= -c_1 \sin x - c_2 \cos x			</mrow>	
	</md>
		
	Now we can substitute into the DE:
	
	<md>
		<mrow>\text{LHS}\amp= \frac{d^2y}{dx^2} + y								</mrow>
		<mrow>			\amp= \Big[ -c_1 \sin x - c_2 \cos x \Big] 
					+ \Big[ c_1 \sin x + c_2 \cos x \Big]		</mrow>
		<mrow>			\amp= 0													</mrow>
		<mrow>			\amp= \text{RHS}										</mrow>	
	</md>
	
	Since when we substitute in to the DE, we find that the LHS is equal to the RHS, 
	we have verified that <m>y = c_1 \sin x + c_2 \cos x</m> is a solution to the DE
	<m>\DS \frac{d^2y}{dx^2} + y = 0.</m>
	</solution>
	<answer>
		Since we get the same result (0) when we substitute the solution into the RHS 
		and into the LHS, we confirm that <m>y = c_1 \sin x + c_2 \cos x</m> is a
		solution to the DE.
	</answer>
	</li>
	<!-- Do we need this?
	<li xml:id="soln_form1"> 
	<p>
	<em> Assuming the form of the solution of DE.</em> 
						<!- from Nagle, Saff and Snider ->
	</p>
	</li>
	-->
	<li> 
	<p>
	Consider the DE 
	
	<men xml:id="soln_form1">\DS \frac{d^2 y}{dx^2} + 6 \frac{dy}{dx} + 5y = 0.</men>
	
	</p>
	
	<p>		
	Find all values of <m>m</m> such that <m>y = e^{mx}</m> is a solution to the DE 
	by taking derivatives and substituting into the DE, and then solving for <m>m</m>.
	</p>
		
	<hint>
		<m>e^{mx} \ne 0,</m> no matter the value of <m>x</m> or <m>m.</m> 
		Therefore we might want to factor it out as it won't contribute to our answer.
	</hint>
	<solution>
	First we take derivatives so that we can substitute into the DE.
	
	<md>
		<mrow>						y	\amp= e^{mx}							</mrow>
		<mrow>	\Rightarrow \quad   y'	\amp= me^{mx}							</mrow>
		<mrow>	\Rightarrow \quad   y''	\amp= m^2 e^{mx}						</mrow>	
	</md> 

	Now we can substitute into the DE and solve for <m>m</m>:

	<md>
		<mrow>\frac{d^2 y}{dx^2} 
				+ 6 \frac{dy}{dx} + 5y	\amp= 0							</mrow>
		<mrow>\Big[ m^2 e^{mx} \Big] + 6\Big[ m e^{mx} \Big] 
				+ 5\Big[ e^{mx} \Big]	\amp= 0							</mrow>
		<mrow>	e^{mx} \Big[ m^2 + 6m + 5 Big]	\amp= 0							</mrow>
		<mrow>				e^{mx} (m+5)(m+1)	\amp= 0							</mrow>	
	</md>
	
	Recall that <m>e^{mx} \ne 0,</m> no matter the value of <m>x</m> or <m>m.</m>
	Thus we have:
	
	<md>
		<mrow>	m+5 = 0 \amp \text{ or } m+1 = 0								</mrow>
		<mrow>	m = -5,	\amp \text{ or } m = -1									</mrow>	
	</md>
	So the two solutions are <m>m = -5, -1.</m>
	</solution>
	<answer>
		<me> m = -5, -1 </me>
	</answer>
	</li>
	<li>
	<p>
	Now that you have (hopefully!) two values for <m>m,</m> choose one of the two values 
	and then verify that <m>y = e^{mx}</m> is a solution for that value of <m>m.</m>
	</p>
	<solution>
	<p>
	The work here is for <m>m = -5,</m> and the work for <m>m = -1</m> is similar.
	</p>
	<p>
	First we take derivatives so that we can substitute into the DE.
	
	<md>
		<mrow>							y	\amp= e^{-5x}						</mrow>
		<mrow>		\Rightarrow \quad   y'	\amp= -5e^{-5x}						</mrow>
		<mrow>		\Rightarrow \quad 	y''	\amp= 25 e^{-5x}					</mrow>	
	</md> 
		
	Now we can substitute into the DE:
	
	<md>
		<mrow>\text{LHS}\amp= \frac{d^2 y}{dx^2} + 6 \frac{dy}{dx} + 5y			</mrow>
		<mrow>			\amp= \Big[ 25e^{-5x} \Big] + 6\Big[ -5e^{-5x} \Big] 
							+ 5\Big[ e^{-5x} \Big]		</mrow>
		<mrow>			\amp= 25e^{-5x} - 30 e^{-5x} + 5e^{-5x}					</mrow>
		<mrow>			\amp= 0													</mrow>
		<mrow>			\amp= \text{RHS}										</mrow>	
	</md>
	
	Hence, we have shown that <m>y = e^{-5x}</m> is a solution to the DE 
	<m>\DS  \frac{d^2 y}{dx^2} + 6 \frac{dy}{dx} + 5y = 0.</m>
	</p>
	</solution>
	<answer>
		Since we get the same result (0) when we substitute the solution into the RHS 
		and into the LHS, we confirm that <m>y = e^{-5x}</m> (or <m>y = e^{-x}</m>) 
		is a solution to the DE.
	</answer>
	</li>
	<li> 
	<!-- Do we need this?
	<p>
	<em> Assuming the form of the solution of DE. </em>
	</p>
	-->
	
	<p>
	Find all values of <m>m</m> such that <m>y = x^m</m> is a solution of the DE 
	
	<men xml:id="soln_form2">\DS 3x^2 \frac{d^2y}{dx^2} = -11x \frac{dy}{dx} + 3y.</men>
	</p>
	<solution>
	<p>
	We proceed as in the previous question. First we take derivatives so that we can substitute into the DE.
	
	<md>
		<mrow>						y	\amp= x^m								</mrow>
		<mrow>	\Rightarrow \quad   y'	\amp= mx^{m-1}							</mrow>
		<mrow>	\Rightarrow \quad   y''	\amp= m(m-1)x^{m-2}						</mrow>	
	</md> 
		
	Now we can substitute into the DE:
	
	<md>
		<mrow>				3x^2 \frac{d^2y}{dx^2}	\amp= 
					-11x \frac{dy}{dx} + 3y						</mrow>
		<mrow>		3x^2\Big[ m(m-1)x^{m-2} \Big]	\amp= 
					-11x\Big[ mx^{m-1} \Big] + 3\Big[ x^m \Big]	</mrow>
		<mrow>					3m(m-1)x^2 x^{m-2}	\amp= 
					-11mx^1\cdot x^{m-1} + 3x^m					</mrow>
		<mrow>				(3m^2 - 3m)x^{2+(m-2)}	\amp= 
					-11m x^{1 + (m-1)} + 3x^m					</mrow>
		<mrow>					(3m^2 - 3m)x^{m}	\amp= -11m x^{m} + 3x^m		</mrow>
		<mrow>(3m^2 - 3m)x^{m} + 11m x^{m} - 3x^m	\amp= 0						</mrow>
		<mrow>			(3m^2 - 3m + 11m - 3)x^m	\amp= 0						</mrow>
		<mrow>					(3m^2 +8m - 3)x^m	\amp= 0						</mrow>
		<mrow>						(3m -1)(m+3)x^m	\amp= 0						</mrow>	
	</md>
	Note that there is no value of <m>m</m> that can guarantee that <m>x^m</m> is 0.
	Hence we have
		
	<md>
		<mrow>			3m-1 = 0 \amp \quad\text{or}\quad m+3 = 0				</mrow>
		<mrow>	m = \frac{1}{3}, \amp \quad\text{or}\quad m = -3				</mrow>	
	</md>
	So the two solutions are <m>m = -3, \frac{1}{3}.</m>
	</p>
	</solution>
	<answer>
		<me> m = -3, \frac{1}{3} </me>
	</answer>
	</li>
	</ol>
</p>

	<p>
		Let's look at a couple of examples to see how this works.
	</p>
	
	<example xml:id="example-de-solution-01">
	
		<p>
		Verify that <m>\DS y = Ce^{x^2} + 3</m>, where <m>C</m> is any constant, is a solution to the DE
		<me>\DS \frac{dy}{dx} = 2xy - 6x.</me>
		</p>
	
		<solution>
	
		<p>
			We'll approach this the same way we approached the algebraic equation in the example above: we will to substitute the function <m>\DS y = Ce^{x^2} + 3</m> in on the left and right hand sides of the equation
	
			<sidebyside widths="45% 55%" margins="auto" valign="top" halign="center">
			<p>
				<md>
				<mrow> \overset{LHS\vphantom{\Big|}}{\frac{dy}{dx}}
					\amp=\frac{d}{dx}\left( Ce^{x^2} + 3 \right)</mrow>
				<mrow> 	\amp= C\frac{d}{dx}\left( e^{x^2} \right) + \frac{d}{dx}\left( 3 \right)</mrow>
				<mrow> 	\amp= C \cdot e^{x^2} \cdot \frac{d}{dx}\left( x^2 \right) + 0</mrow>
				<mrow> 	\amp=  C \cdot e^{x^2} \cdot 2x</mrow>
				<mrow> 	\amp=  2Cxe^{x^2}</mrow>
				</md>
			</p>
			<p>
				<md>
				<mrow> 	\overset{RHS\vphantom{\Big|}}{2xy - 6x}
					\amp= 2x \left( Ce^{x^2} + 3 \right) - 6x</mrow>
				<mrow> 	\amp= 2Cxe^{x^2} + 6x - 6x</mrow>
				<mrow> 	\amp= 2Cxe^{x^2}</mrow>
				</md>
			</p>
			</sidebyside>
	
			Since both the <m>LHS</m> and <m>RHS</m> turn out to be	<m>2Cxe^{x^2}</m>, we have shown that <m>\DS y = Ce^{x^2} + 3</m> satisfies and is, thus, a	solution to	<m>\DS \frac{dy}{dx} = 2xy - 6x.</m>
		</p>
	
		</solution>
	
	</example>
	
	<p>
		Since we used a generic constant <m>C</m>, we have shown that <m>\DS y = Ce^{x^2} + 3</m> is a solution for any value we like for the constant <m>C</m>. In particular,
		<ul>
		<li>for <m>C=-41, \quad y = -41e^{x^2} + 3 \quad</m> is a solution.</li>
		<li>for <m>C=199, \quad y = 199e^{x^2} + 3 \quad</m> is a solution.</li>
		<li>for <m>C=0, \quad y = 3 \quad</m> is a solution.</li>
		</ul>
		Since there is no limit to what <m>C</m> we can choose, this DE must have an infinite number of solutions. In the next section, we will describe this idea further.
	</p>

	<example xml:id="example-de-solution-05">
	
		<p>
		Determine if <m>y = c_1e^{-3t} + c_2e^{4t}</m> is a solution to the DE
		<m>y'' - y' - 12y = 0</m> where <m>c_1</m> and <m>c_2</m> are constants.
		</p>
	
		<solution>
		<p>
			Find <m>y, y', \text{ and } y''</m>.
			<md>
			<mrow>y		\amp= c_1e^{-3t} + c_2e^{4t} \hspace{-0.4cm}
				\amp\Rightarrow\hspace{0.1cm}
				y'	\amp= -3c_1e^{-3t} + 4c_2e^{4t} \hspace{-0.4cm}
				\amp\Rightarrow\hspace{0.1cm}
				y''	\amp= 9c_1e^{-3t} + 16c_2e^{4t}
			</mrow>
			</md>
		</p>
	
		<p>
			and substitute
			<md>
			<mrow>LHS	\amp= y'' - y' - 12y										</mrow>
			<mrow>		\amp= \left(9c_1e^{-3t} + 16c_2e^{4t}\right)
				- \left( -3c_1e^{-3t} + 4c_2e^{4t} \right)
				- 12\left( c_1e^{-3t} + c_2e^{4t} \right)				</mrow>
			<mrow>		\amp= 9c_1e^{-3t} + 16c_2e^{4t} + 3c_1e^{-3t}
				- 4c_2e^{4t} - 12c_1e^{-3t} - 12c_2e^{4t}			</mrow>
			<mrow>		\amp= \left( 9c_1e^{-3t} + 3c_1e^{-3t} - 12c_1e^{-3t} \right)
				+ \left( 16c_2e^{4t} - 4c_2e^{4t} - 12c_2e^{4t} \right)	</mrow>
			<mrow>		\amp = 0													</mrow>
			<mrow>		\amp= RHS													</mrow>
			</md>
			Which shows that <m>y = c_1e^{-3t} + c_2e^{4t}</m> is a solution to <m>y'' - y' - 12y = 0.</m>
		</p>
	
		</solution>
	
	</example>
	
	<example xml:id="example-de-solution-06">
	
		<statement>
			<p>
				Verify that <m>y = Ce^{-5x^2} + \frac{3}{5}</m> is a solution to the DE
				<me>\frac{dy}{dx} = \big( 2x \big) \big( 3 - 5y \big)</me>
			</p>
		</statement>
	
		<solution>
			<p>
				Working out the left and right hand sides of this DE, we have:
	
				<sidebyside widths="45% 55%" margins="auto" valign="top" halign="center">
				<p>
					<md>
						<mrow> LHS: </mrow>
						<mrow> \frac{dy}{dx}
								\amp=\frac{d}{dx}\left( Ce^{-5x^2} + \frac{3}{5} \right)</mrow>
						<mrow> 	\amp= Ce^{-5x^2} \cdot \frac{d}{dx}(-5x^2) + 0</mrow>
						<mrow> 	\amp= Ce^{-5x^2} \cdot -10x</mrow>
						<mrow> 	\amp= -10Cxe^{-5x^2}</mrow>
					</md>
				</p>
				<p>
					<md>
						<mrow> RHS: </mrow>
						<mrow> 	\big(2x\big)\amp\big(3 - 5y\big)</mrow>
						<mrow> 	\amp= 2x \left[3 - 5\left(Ce^{-5x^2} + \frac{3}{5}\right) \right]</mrow>
						<mrow> 	\amp= 2x \left[ 3 - 5Ce^{-5x^2} - 3 \right]</mrow>
						<mrow> 	\amp= 2x \left[-5Ce^{-5x^2}\right]</mrow>
						<mrow> 	\amp= -10Cxe^{-5x^2}</mrow>
					</md>
				</p>
				</sidebyside>
			</p>
	
			<p>
				Since <m>LHS = RHS</m>, we have verified that
				<m>y = Ce^{-5x^2} + \frac{3}{5}</m> is a solution to
				<me>\frac{dy}{dx} = \big( 2x \big) \big( 3 - 5y \big)</me>
			</p>
		</solution>
	
	</example>
	
	<p>
		Edit Notes:
		<ul>
		<li> perhaps add concluding thought to the progression of examples that showed linear combinations of solutions were also a solution in this particular case? Or just wait until the next subsection? </li>
		</ul>
	</p>


	<xi:include href="./p1-c2-s2-interactives.ptx" />
	<xi:include href="./p1-c2-s2-exercises.ptx" />

</section>