<section><title> Orphaned Content </title>

    <introduction>
        <p>
            This is just a place to put content that was written and may or not be used.
        </p>
    </introduction>

	<subsection xmlns:xi="http://www.w3.org/2001/XInclude"><title> Types of Solutions </title>

		<p>
			We have just discussed some important ideas that will aid us in understanding what it means to be a solution to an differential equation. You will see that the next two statement are practically identical (except the blue terms).
		</p>
	
		<ul>
			<li>
				<m>\color{blue}{x}</m> (a <m>\color{blue}{\text{number}}</m>) is a solution to an <m>\color{blue}{\text{algebraic}}</m> equation if we get the same result on the left and right-hand side of the equation after substituting <m>\color{blue}{x}</m> into the entire equation.
			</li>
			<li>
				<m>\color{blue}{y}</m> (a <m>\color{blue}{\text{function}}</m>) is a solution to a <m>\color{blue}{\text{differential}}</m> equation if we get the same result on the left and right-hand side of the equation after substituting <m>\color{blue}{y}</m> into the entire equation.
			</li>
		</ul>
		
		
		<p>
			Recall, <m>\color{blue}{x}</m> (a <m>\color{blue}{\text{number}}</m>) is a solution to an <m>\color{blue}{\text{algebraic}}</m>	equation if:
			<sidebyside widths="90%" margins="auto" valign="middle">
			<p>
				If we get the same result on the left and right-hand side of the equation after plugging <m>\color{blue}{x}</m> into the entire equation, then we say <m>\color{blue}{x}</m> is a solution to the <m>\color{blue}{\text{algebraic}}</m> equation.
			</p>
			</sidebyside>
		</p>
		<p>
			Similarly, <m>\color{blue}{y}</m> (a <m>\color{blue}{\text{function}}</m>) is a solution to an <m>\color{blue}{\text{differential}}</m> equation if:
			<sidebyside widths="90%" margins="auto" valign="middle">
			<p>
				If we get the same result on the left and right-hand side of the equation after plugging <m>\color{blue}{y}</m> into the entire equation, then we say <m>\color{blue}{y}</m> is a solution to the <m>\color{blue}{\text{differential}}</m> equation.
			</p>
			</sidebyside>
		</p>
		
		
	
		<p>
			In all of the previous examples, we verified that one particular function was a solution to the DE, but as previously mentioned, we know that there may be more. It turns out, differential equations generally have infinitely many solutions. We can use <xref ref="example-de-solution-05" /> to illustrate this.
		</p>
	
		<p>
			In this example, we showed that the function <m>y = c_1e^{-3t} + c_2e^{4t}</m> was a solution <m>y'' - y' - 12y = 0</m>.
		</p>
	
		<p>
			Notice that we were able to verify the solution, even though the constants, <m>c_1</m> and <m>c_2</m>, were not known. This suggests that you can substitute any values of <m>c_1</m> and <m>c_2</m> into the solution and it will still be a solution to the DE. <em> Try it! </em>
		</p>
	
		<p>
			Now, since there are infinitely many choices for <m>c_1</m> and <m>c_2</m>,	then, logically, there must be infinitely many solutions to the DE,	<m>y'' - y' - 12y = 0</m>.
		</p>
	
	</subsection>

	<paragraphs><title> Additional Examples </title>

        <example xml:id="calculus-pov"><title> A Calculus Perspective </title>
			
            <p>
                Suppose you were given <m> y(t) = 4t^3 + \sin t </m>, and asked to find <m>y''</m>.
            </p>
        
            <p/>
        
            <p>
                Since we are familiar with calculus, we quickly take two derivatives of <m>y</m>, giving
                <md>
                    <mrow> y' 	\amp= 12t^2	+ \cos t		</mrow>
                    <mrow> y'' 	\amp= 24t 	- \sin t.		</mrow>
                </md>
            </p>
        
            <p>
                This task is no problem for us, but suppose we started with
                <me> y'' = 24t 	- \sin t	</me>
                and were asked to go in the reverse direction. That is, find a function, <m>y(t)</m>, that has <m>24t - \sin t</m> as a second derivative. <em> This is precisely what solving a differential equation aims to do and we would phrase this problem as, </em>
            </p>
    
            <sidebyside widths="80%" halign="center" valign="bottom">
                <p>
                    "given the differential equation, <m> y'' = 24t 	- \sin t</m>, solve for <m>y.</m>"
                </p>
            </sidebyside>
            
            </example>
        
            <example xml:id="physics-pov"><title> A Physics Perspective </title>
            <p>
                Let <m>y(t)</m> be the position of some object at time, <m>t</m>.  Assume for the moment that we don't know what <m>y</m> is, but we do know the object is moving with a constant velocity of <m>4.6</m> meters per second.
            </p>  
                
            <p>
                Physics tells us that velocity is the rate of change of position (i.e., derivative of position, <m>y'(t)</m>). So, given that the object is moving at a known constant velocity, we may write
                <me> y'(t) = 4.6. </me>
            </p>
        
            <p>
                This is another example of a differential equation where one could ask "what function, <m>y(t)</m>, has a derivative that is equal to <m>4.6</m>?"
            </p>
        
            </example>
        
            <p> 
                The situations above illustrate simple examples of what a differential differential equation is and what it means to "solve" a differential equation. Throughout this text, we will present many more examples and discuss various techniques used to solve them. 
            </p>

			<p>
				Let's look at a couple of examples to see how this works.
			</p>
			
			<example xml:id="example-de-solution-01">
			
				<p>
					Verify that <m>\DS y = Ce^{x^2} + 3</m>, where <m>C</m> is any constant, is a solution to the DE
					<me>\DS \frac{dy}{dx} = 2xy - 6x.</me>
				</p>
			
				<solution>
			
					<p>
						We'll approach this the same way we approached the algebraic equation in the example above: we will to substitute the function <m>\DS y = Ce^{x^2} + 3</m> in on the left and right hand sides of the equation
				
						<sidebyside widths="45% 55%" margins="auto" valign="top" halign="center">
							<p>
								<md>
								<mrow> \overset{LHS\vphantom{\Big|}}{\frac{dy}{dx}}
									\amp=\frac{d}{dx}\left( Ce^{x^2} + 3 \right)</mrow>
								<mrow> 	\amp= C\frac{d}{dx}\left( e^{x^2} \right) + \frac{d}{dx}\left( 3 \right)</mrow>
								<mrow> 	\amp= C \cdot e^{x^2} \cdot \frac{d}{dx}\left( x^2 \right) + 0</mrow>
								<mrow> 	\amp=  C \cdot e^{x^2} \cdot 2x</mrow>
								<mrow> 	\amp=  2Cxe^{x^2}</mrow>
								</md>
							</p>
							<p>
								<md>
								<mrow> 	\overset{RHS\vphantom{\Big|}}{2xy - 6x}
									\amp= 2x \left( Ce^{x^2} + 3 \right) - 6x</mrow>
								<mrow> 	\amp= 2Cxe^{x^2} + 6x - 6x</mrow>
								<mrow> 	\amp= 2Cxe^{x^2}</mrow>
								</md>
							</p>
						</sidebyside>
				
						Since both the <m>LHS</m> and <m>RHS</m> turn out to be	<m>2Cxe^{x^2}</m>, we have shown that <m>\DS y = Ce^{x^2} + 3</m> satisfies and is, thus, a	solution to	<m>\DS \frac{dy}{dx} = 2xy - 6x.</m>
					</p>
			
				</solution>
			
			</example>
			
			<p>
				Since we used a generic constant <m>C</m>, we have shown that <m>\DS y = Ce^{x^2} + 3</m> is a solution for any value we like for the constant <m>C</m>. In particular,
				<ul>
				<li>for <m>C=-41, \quad y = -41e^{x^2} + 3 \quad</m> is a solution.</li>
				<li>for <m>C=199, \quad y = 199e^{x^2} + 3 \quad</m> is a solution.</li>
				<li>for <m>C=0, \quad y = 3 \quad</m> is a solution.</li>
				</ul>
				Since there is no limit to what <m>C</m> we can choose, this DE must have an infinite number of solutions. In the next section, we will describe this idea further.
			</p>
		
			<example xml:id="example-de-solution-05">
			
				<p>
					Determine if <m>y = c_1e^{-3t} + c_2e^{4t}</m> is a solution to the DE <m>y'' - y' - 12y = 0</m> where <m>c_1</m> and <m>c_2</m> are constants.
				</p>
			
				<solution>
		
					<p>
						Find <m>y, y', \text{ and } y''</m>.
						<md>
							<mrow>y		\amp= c_1e^{-3t} + c_2e^{4t} \hspace{-0.4cm}
								\amp\Rightarrow\hspace{0.1cm}
								y'	\amp= -3c_1e^{-3t} + 4c_2e^{4t} \hspace{-0.4cm}
								\amp\Rightarrow\hspace{0.1cm}
								y''	\amp= 9c_1e^{-3t} + 16c_2e^{4t}
							</mrow>
						</md>
					</p>
				
					<p>
						and substitute
						<md>
							<mrow>LHS	\amp= y'' - y' - 12y										</mrow>
							<mrow>		\amp= \left(9c_1e^{-3t} + 16c_2e^{4t}\right)
								- \left( -3c_1e^{-3t} + 4c_2e^{4t} \right)
								- 12\left( c_1e^{-3t} + c_2e^{4t} \right)				</mrow>
							<mrow>		\amp= 9c_1e^{-3t} + 16c_2e^{4t} + 3c_1e^{-3t}
								- 4c_2e^{4t} - 12c_1e^{-3t} - 12c_2e^{4t}			</mrow>
							<mrow>		\amp= \left( 9c_1e^{-3t} + 3c_1e^{-3t} - 12c_1e^{-3t} \right)
								+ \left( 16c_2e^{4t} - 4c_2e^{4t} - 12c_2e^{4t} \right)	</mrow>
							<mrow>		\amp = 0													</mrow>
							<mrow>		\amp= RHS													</mrow>
						</md>
						Which shows that <m>y = c_1e^{-3t} + c_2e^{4t}</m> is a solution to <m>y'' - y' - 12y = 0.</m>
					</p>
			
				</solution>
			
			</example>
			
			<example xml:id="example-de-solution-06">
			
				<statement>
					<p>
						Verify that <m>y = Ce^{-5x^2} + \frac{3}{5}</m> is a solution to the DE
						<me>\frac{dy}{dx} = \big( 2x \big) \big( 3 - 5y \big)</me>
					</p>
				</statement>
			
				<solution>
					<p>
						Working out the left and right hand sides of this DE, we have:
			
						<sidebyside widths="45% 55%" margins="auto" valign="top" halign="center">
							<p>
								<md>
									<mrow> LHS: </mrow>
									<mrow> \frac{dy}{dx}
											\amp=\frac{d}{dx}\left( Ce^{-5x^2} + \frac{3}{5} \right)</mrow>
									<mrow> 	\amp= Ce^{-5x^2} \cdot \frac{d}{dx}(-5x^2) + 0</mrow>
									<mrow> 	\amp= Ce^{-5x^2} \cdot -10x</mrow>
									<mrow> 	\amp= -10Cxe^{-5x^2}</mrow>
								</md>
							</p>
							<p>
								<md>
									<mrow> RHS: </mrow>
									<mrow> 	\big(2x\big)\amp\big(3 - 5y\big)</mrow>
									<mrow> 	\amp= 2x \left[3 - 5\left(Ce^{-5x^2} + \frac{3}{5}\right) \right]</mrow>
									<mrow> 	\amp= 2x \left[ 3 - 5Ce^{-5x^2} - 3 \right]</mrow>
									<mrow> 	\amp= 2x \left[-5Ce^{-5x^2}\right]</mrow>
									<mrow> 	\amp= -10Cxe^{-5x^2}</mrow>
								</md>
							</p>
						</sidebyside>
					</p>
			
					<p>
						Since <m>LHS = RHS</m>, we have verified that
						<m>y = Ce^{-5x^2} + \frac{3}{5}</m> is a solution to
						<me>\frac{dy}{dx} = \big( 2x \big) \big( 3 - 5y \big)</me>
					</p>
					
				</solution>
			
			</example>
			
			<p>
				Edit Notes:
				<ul>
					<li> perhaps add concluding thought to the progression of examples that showed linear combinations of solutions were also a solution in this particular case? Or just wait until the next subsection? </li>
				</ul>
			</p>

	</paragraphs>
	
	<reading-questions><title> Additional Practice </title>

        
    
    </reading-questions>

    <paragraphs xml:id="algebra-pov"><title> Algebra </title>
		<p>
			When given an algebraic equation such as <m>x^3 - 6x = 4</m>, the solution is all <em>numbers</em>, <m>x</m>, that satisfy the equation. One such solution is <m>x=-2</m>. This can be verified by plugging <m>x=-2</m> into the equation. After simplifying, if the value on the left equals the value on the right, the solution must be valid. When this happens, we say that the solution "satisfies" this equation.
			<sidebyside widths="40% 40%" margin="0%" valign="bottom">
			
			<p>
				<md>
				<mrow>                            x^3 - 6x  \amp = 4 </mrow>
				<mrow> \left(-2\right)^3 - 6\left(-2\right) \amp = 4 </mrow>
				<mrow>                              -8 + 12 \amp = 4 </mrow>
				<mrow>                                    4 \amp = 4 \, \checkmark </mrow>
				</md>  
			</p>
			
			<p>
				The number, <m>x=-2</m>, is a solution since it "satisfies" this equation.
			</p>
			
			</sidebyside>
		</p>

		<p>
			In contrast, when solving a differential equation such as <m>y' - 6y = 10x - 5</m>, we are looking for all <em>functions</em>, <m>y</m>, that satisfy the equation. One solution is <m>y = -5x</m> and we can verify it in the same way.

			<sidebyside widths="50% 30%" valign="bottom">
			
			<p>
				<md>
				<mrow>                                      y' - 2y   \amp = 10x - 5 </mrow>
				<mrow> \left(-5x\right)^{\prime} - 2\left(-5x\right)  \amp = 10x - 5 </mrow>
				<mrow>                                      -5 + 10x  \amp = 10x - 5 </mrow>
				<mrow>                                        10x - 5 \amp = 10x - 5 \, \checkmark </mrow>
				</md>
			</p>
			
			<p>
				The function, <m>y = -5x</m>, is a solution since it "satisfies" this equation.
			</p>
			
			</sidebyside>

		</p>
			
		</paragraphs>

		<paragraphs><title> An Analogy </title>
		<p>
			It is helpful to make an analogy here by thinking about what it means to be a solution to an algebraic equation. Consider (<em> but don't solve!</em>) the following problem and think about the questions that follow.
		</p>

		<p>
			What does it mean when we say <m>x = -1</m> is a solution to the equation below?
			<me> x^5 + 12x^2 +10x = 7x^3 + 24 </me>
		</p>

		<question>
			<title>What does solution mean in this case?</title>

			<p>
			In the context of this equation, a solution would be an <m>x</m>-value that "works" when we substitute it back into the equation (i.e. it satisfies the equation). If we substitute <m>x = -1</m> into each side of the equation, we have
			<md>
				<mrow>\mbox{left hand side of the equation (LHS)}	%\amp= x^5 + 12x^2 +10x,</mrow>
				<mrow>							\amp= (-1)^5 + 12(-1)^2 +10(-1),</mrow>
				<mrow>							\amp= -1 + 12 - 11,</mrow>
				<mrow>							\amp= 0,</mrow>
			</md>
			and
			<md>
				<mrow>\mbox{right hand side of the equation (RHS)}	%\amp= 7x^3 + 24,</mrow>
				<mrow>								\amp= 7(-1)^3 + 24,</mrow>
				<mrow>								\amp= -7 + 24,</mrow>
				<mrow>								\amp= 17.</mrow>
			</md>
			</p>

			<p>
			When we substitute <m>x = -1</m> into the left hand side of the equation we get <m>0</m>, whereas we get <m>17</m> on the right hand side. This means <m>x = -1</m> isn't a solution to the algebraic equation. However, if we try <m>x = -3,</m> we have
			<md>
				<mrow>\mbox{LHS}	%\amp= x^5 + 12x^2 +10x,</mrow>
				<mrow>							\amp= (-3)^5 + 12(-3)^2 +10(-3),</mrow>
				<mrow>							\amp= -243 + 108 - 30,</mrow>
				<mrow>							\amp= -165,</mrow>
			</md>
			and
			<md>
				<mrow>\mbox{RHS}	%\amp= 7x^3 + 24,</mrow>
				<mrow>								\amp= 7(-3)^3 + 24,</mrow>
				<mrow>								\amp= -189 + 24,</mrow>
				<mrow>								\amp= -165.</mrow>
			</md>
			</p>

			<p>
			Since we get the same result when we substitute <m>x = -3</m> in on the left hand and right hand sides of the equation, we can conclude that <m>x = -3</m> is a solution to the algebraic equation.
			</p>

		</question>

		<p>
			Let's take a moment to highlight some important details about how the previous example gives insight into the concept of a solution to a differential equation.
		</p>

		<ul>
			<li>
			Your intuition for algebra should tell you that there is probably more solutions than <m>x = -3</m> to this equation (and you'd be correct). It turns out that differential equations also can have multiple solutions!
			</li>
			<li>
			At no point did we discuss the technique needed to find the solution <m>x = -3</m>. However, this did not stop us from verifying that it was a solution. This fact also transfers to differential equations! Indeed, as you will see in the exercises, given a function, you will be able to verify whether this function is (or is not) a solution to a differential equation.
			</li>
		</ul>

		</paragraphs>

</section>