<section xmlns:xi="http://www.w3.org/2001/XInclude"><title> Verifying Solutions </title>

    <p>
		Regardless what kind of equation you are working with, a solution is a value or function that <q>satisfies</q> the equation. The term <em>satisfies</em> simply means that when you plug the value into the equation, it simplifies to a statement that is undeniably true. For example, suppose I want to check if <m>y=2</m> and <m>y = 0</m> are solutions to the equation 
		<me>
			y^3 = 3y + 2 
		</me>.
		To do this, we verify that <m>2</m> and <m>0</m> individually <em>satisfy</em> the equation by plugging <m>2</m> and <m>0</m> into each <m>y</m>, simplify and see if we end up with an undeniably true statement, like so
		<sidebyside>
			<p>
				<md>
					<mrow> (2)^3 	=\amp\ 3(2) + 2								</mrow>
					<mrow> 8 		=\amp\ 6 + 2								</mrow>
					<mrow> 8 		=\amp\ 8	\quad \leftarrow \text{true}	</mrow>
				</md>
			</p>
			<p>
				<md>
					<mrow> (0)^3 	=\amp\ 3(0) + 2								</mrow>
					<mrow> 0 		=\amp\ 0 + 2								</mrow>
					<mrow> 0 		=\amp\ 2	\quad \leftarrow \text{false}	</mrow>
				</md>
			</p>
		</sidebyside>
		Since <m>y=2</m> satisfies the equation, but <m>y=0</m> does not, we can only say that <m>y=2</m> is a solution.
	</p>

	<p>
		The same idea applies to differential equations, except in that solutions are functions instead of numbers. To see this, let's verify if <m>y = 3x</m> and <m>y = e^{3x}</m> are solutions to the differential equation
		<m>
			\displaystyle y^\prime = 3y
		</m>.
	</p>

	<p>
		As before, we plug-in <m>3x</m> and <m>e^{3x}</m> for each <m>y</m> and simplify.
		<sidebyside>
			<p>
				<md>
					<mrow> \left[3x\right]^\prime 	=\amp\ 3(3x)								</mrow>
					<mrow> 3 						=\amp\ 9x	\quad \leftarrow \text{false}	</mrow>
				</md>
			</p>
			<p>
				<md>
					<mrow> \left[e^{3x}\right]^\prime 			=\amp\ 3e^{3x}									</mrow>
					<mrow> e^{3x} \cdot \left[3x\right]^\prime	=\amp\ 3e^{3x}									</mrow>
					<mrow> e^{3x} \cdot 3						=\amp\ 3e^{3x}									</mrow>
					<mrow> 3e^{3x}								=\amp\ 3e^{3x}	\quad \leftarrow \text{true}	</mrow>
				</md>
			</p>
		</sidebyside>
		Since <m>y=3x</m> results in a false statement, it does not satisfy the equation and is not a solution. However, since <m>y=e^{3x}</m> satisfies the equation, it is a solution.
	</p>

	<p>
		<assemblage color="green" xml:id="solution-verification-steps"><title>Solution Verification Steps</title>
			<p>
				Verifying if a function is a solution to a differential equation involves checking if the function satisfies the equation, outlined as follows:
				<dl width="narrow">
					<li xml:id="solution-verification-compute"><title>Compute</title>
						<line> 
							Compute &amp; simplify derivatives appearing in the DE
							<fn> This helps reduce errors by breaking the problem into more manageable steps. </fn>
						</line>
					</li>
					<li xml:id="solution-verification-substitute"><title>Substitute</title>
						<p> 
							Substitute the function &amp; derivatives into the equation
						</p>
					</li>
					<li xml:id="solution-verification-simplify"><title>Simplify</title>
						<p> 
							Simplify the left &amp; right hand sides of the equation
						</p>
					</li>
				</dl>
				If you end up with a true statement, then the function is a solution.
			</p>
		</assemblage>
	</p>

	<example><title> <em>Solution Verification 1</em> </title>
		<p>
			Is <m>y= 2x^2</m> a solution to the DE <m>\quad xy' - 2y = x</m>?
		</p>

		<solution>

			<p>
				Let's follow the steps outlined above.
			</p>

			<p>
				<xref ref="solution-verification-compute" text="title"/> <m>y'</m> since it appears in the DE.
				<me>
					y	= 2x^2,	\quad	y' = 4x
				</me>
			</p>

			<p>
				<p>
				<xref ref="solution-verification-substitute" text="title"/> <m>y</m> and <m>y'</m> into the DE.
				</p>
				<sidebyside widths="85% 15%">
					<p>
						<md>
							<mrow> xy' - 2x^2	\amp= y	</mrow>
							<mrow> 4x^2 - 2x^2 	\amp= \left( 2x^2 \right) </mrow>
							<mrow> 
								<xref ref="solution-verification-simplify" text="title"/> \hspace{2.2cm}
								4x^2 - 2x^2	\amp= 2x^2
							</mrow>
							<mrow> 2x^2	\amp= 2x^2	\quad \leftarrow \text{true}	</mrow>
						</md>
					</p>
					<p/>
				</sidebyside>
				Therefore, <m>y= 2x^2</m> is <term> not a solution </term> to <m>y' - 2xy = x.</m>
			</p>

		</solution>

	</example>

	<example><title> <em>Solution Verification 2</em> </title>
		<p>
			Is <m>y= 2e^{-3t}</m> a solution to the DE <m>\quad y'' - y' - 12y = 0</m>?
		</p>

		<solution><title><xref ref="solution-verification-compute" text="title"/></title>
		
		

			<tabular top="major">
				<col width="20%" />
				<col width="80%" />
				<row valign="top" bottom="medium">
				  <cell>Unit</cell>
				  <cell>Definition</cell>
				</row>
				<row valign="top" bottom="minor">
				  <cell><xref ref="solution-verification-compute" text="title"/></cell>
				  <cell>
						<md>
							<mrow>	y	\amp=  2e^{-3t}	</mrow>
							<mrow>	y' 	\amp=  2e^{-3t}\left(-3\right) \quad \rightarrow y' =  -6e^{-3t}</mrow>
							<mrow>	y'' \amp= -6e^{-3t}\left(-3\right) \quad \rightarrow y'' = 18e^{-3t}</mrow>
						</md>
				  </cell>

				</row>
				<row valign="top" bottom="minor">
				  <cell><quantity>
					  <unit base="minute" />
					</quantity></cell>
				  <cell>
					<p>
					  exactly <m>60</m> seconds
					</p>
				  </cell>

				</row>
				<row valign="top" bottom="major">
				  <cell><quantity>
					  <unit base="hour" />
					</quantity></cell>
				  <cell>
					<p>
					  exactly <m>3600</m> seconds;
					  exaclty <m>60</m> minutes
					</p>
				  </cell>
	
				</row>
			  </tabular>

			  </solution>

			<solution>
			<p>
				<xref ref="solution-verification-compute" text="title"/> <m>y'</m> and <m>y''</m> since they appear in the DE.
				<md>
					<mrow>	y	\amp=  2e^{-3t}	</mrow>
					<mrow>	y' 	\amp=  2e^{-3t}\left(-3\right) \quad \rightarrow y' =  -6e^{-3t}</mrow>
					<mrow>	y'' \amp= -6e^{-3t}\left(-3\right) \quad \rightarrow y'' = 18e^{-3t}</mrow>
				</md>

			<tabular>
				<col width="20%" />
				<col width="40%" />
				<col width="20%" />
				<col width="20%" />
				<row>
					<cell><p><xref ref="solution-verification-compute" text="title"/></p></cell>
					<cell><p><m>y'</m> and <m>y''</m> since they appear in the DE.</p></cell>
					<cell><p>q</p></cell>
					<cell><p>q</p></cell>
				</row>
				<row>
					<cell><p></p></cell>
					<cell><p><md>
						<mrow>	y	\amp=  2e^{-3t}	</mrow>
						<mrow>	y' 	\amp=  2e^{-3t}\left(-3\right) \quad \rightarrow y' =  -6e^{-3t}</mrow>
						<mrow>	y'' \amp= -6e^{-3t}\left(-3\right) \quad \rightarrow y'' = 18e^{-3t}</mrow>
					</md></p></cell>
					<cell><p>q</p></cell>
					<cell><p>q</p></cell>
				</row>
			</tabular>
		</p>

			<p>
				<dl width="narrow">
					<li>
						<title>Substitute</title>
						<p>
							<m>y, y',</m> and <m>y''</m> into the DE
							<md>
								<mrow> 
									y'' - y' - 12y	\amp= 0	
								</mrow>
								<mrow> 
									18e^{-3t} - \left( -6e^{-3t} \right) - 12\left( 2e^{-3t} \right)	\amp= 0 
								</mrow>
							</md>
						</p>
					</li>
					<li>
						<title>Simplify</title>
						<p>
							<md>
								<mrow> 
									18e^{-3t} + 6e^{-3t} - 24e^{-3t}	\amp= 0	
								</mrow>
								<mrow> 
									0	\amp= 0	\quad \leftarrow \text{true}
								</mrow>
							</md>
						</p>
					</li>
				</dl>
				<p>
				<xref ref="solution-verification-substitute" text="title"/> <m>y, y',</m> and <m>y''</m> into the DE.
				</p>
				<sidebyside widths="85% 15%">
					<p>
						<md>
							<mrow> 
								y'' - y' - 12y	\amp= 0	
							</mrow>
							<mrow> 
								18e^{-3t} - \left( -6e^{-3t} \right) - 12\left( 2e^{-3t} \right)	\amp= 0 
							</mrow>
							<mrow> 
								<xref ref="solution-verification-simplify" text="title"/> \hspace{2.2cm}
								18e^{-3t} + 6e^{-3t} - 24e^{-3t}	\amp= 0	
							</mrow>
							<mrow> 
								0	\amp= 0	\quad \leftarrow \text{true}
							</mrow>
						</md>
					</p>
					<p/>
				</sidebyside>
				Therefore, <m>y= 2e^{-3t}</m> is a solution to <m>y'' - y' - 12y = 0.</m>
			</p>

		</solution>

	</example>

	<example>

		<p>
			Determine if <m>y = e^{4t}</m> is a solution to the DE <m>y'' - y' - 12y = 0</m>.
		</p>

		<solution>

		<p>
			<md>
				<mrow>	y	\amp= e^{4t} 	\hspace{-0.4cm}\amp\Rightarrow \hspace{0.1cm}
					y'	\amp= 4e^{4t}	\hspace{-0.4cm}\amp\Rightarrow \hspace{0.1cm}
					y''	\amp= 16e^{4t}
				</mrow>
			</md>

			<md>
				<mrow>LHS	\amp= y'' - y' - 12y									</mrow>
				<mrow>		\amp= \left(16e^{4t}\right) - \left( 4e^{4t} \right)
					- 12\left( e^{4t} \right)			</mrow>
				<mrow>		\amp= 16e^{4t} - 4e^{4t} - 12e^{4t}						</mrow>
				<mrow>		\amp= 0													</mrow>
				<mrow>		\amp= RHS												</mrow>
			</md>
			So, yes, <m>y = e^{4t}</m> is a solution to <m>y'' - y' - 12y = 0.</m>
		</p>

		</solution>

	</example>

	<example>
		
		<p>
			Verify that <m>\DS y = 3\sin(x^2)</m> is a solution to the DE
			<me>y' - 12x^2\sin(x^2) = xy''</me>.
		</p>

		<solution>

			<p>
				First, let's compute <m>y'</m> and <m>y''</m> since we will need to plug them into the DE.
				<md>
					<mrow>y'	\amp= \frac{d}{dx}\left( 3\sin(x^2) \right)</mrow>
					<mrow>		\amp= 3\cos(x^2) \cdot \frac{d}{dx}\left( x^2\right) \hspace{0.2cm}\mbox{(using the chain rule)}</mrow>
					<mrow>		\amp= 3\cos(x^2) \cdot 2x</mrow>
					<mrow>		\amp= 6x\cos(x^2)</mrow>
					<mrow>		\amp</mrow>
					<mrow>y''	\amp= 6x \cdot \frac{d}{dx}\left( \cos(x^2) \right) + \frac{d}{dx}\left( 6x \right)\cdot \cos(x^2) \hspace{0.2cm} \mbox{(using the product rule)}</mrow>
					<mrow>		\amp= -12x^2\sin(x^2) + 6\cos(x^2)</mrow>
				</md>
			</p>

			<p>
				With these in hand, we can substitute into the left and right hand sides of the equation, as follows.
				<md>
					<mrow>\mbox{LHS} 	\amp= y' - 12x^2\sin(x^2) </mrow>
					<mrow>						\amp= 6x\cos(x^2) - 12x^2\sin(x^2)</mrow>
					<mrow> 						\amp</mrow>
					<mrow>\mbox{RHS} 	\amp= xy'' 	</mrow>
					<mrow>						\amp= x\left( -12x^2\sin(x^2) + 6\cos(x^2) \right)</mrow>
					<mrow> 						\amp= -12x^3\sin(x^2) + 6x\cos(x^2)</mrow>
				</md>
			</p>

			<p>
				The resulting expressions left hand side and the right hand side are similar, but they are not the same. Hence,
				<m>y = 3\sin(x^2)</m> is <term> not a solution </term> to <m>y' - 12x^2\sin(x^2) = xy''</m>.
			</p>

		</solution>

	</example>

	<xi:include href="./p1-c2-s1-interactives.ptx" />

</section>