<subsection xmlns:xi="http://www.w3.org/2001/XInclude"><title> Additional Examples </title>

	<example><title> <em>Solution Verification 5</em> </title>
		<p>
			Is <m>y= 3\sin(x^2)</m> a solution to the DE <m>\quad y' - 12x^2\sin(x^2) = xy''</m>?
		</p>

		<solution>

			<p>
				<xref ref="solution-verification-step-1" text="title"/>. Find <m>y'</m> and <m>y''</m> since they appear in the DE.
				<md>
					<mrow>	y	\amp=  3\sin(x^2)									</mrow>
					<mrow>	y' 	\amp=  3\cos(x^2) \cdot 2x	=	6x\cos(x^2)	</mrow>
					<mrow>	y'' \amp= 6\cos(x^2) - 12x\sin(x^2)	=	6\cos(x^2) - 12x\sin(x^2)	</mrow>
				</md>
			</p>

			<p>
				<xref ref="solution-verification-step-2" text="title"/>. Plug <m>y, y',</m> and <m>y''</m> into the DE and simplify.
				<md>
					<mrow> 													y' - 12x^2\sin(x^2)	\amp= xy''									</mrow>
					<mrow> 6x\cos(x^2) - 12x^2\sin(x^2)	\amp= x\left( 6\cos(x^2) - 12x\sin(x^2) \right)	</mrow>
					<mrow> 6x\cos(x^2) - 12x^2\sin(x^2)	\amp= 6x\cos(x^2) - 12x^2\sin(x^2)	</mrow>
					<mrow> 0	\amp= 0	\quad \leftarrow \text{true}	</mrow>
				</md>
				Therefore, <m>y= 3\sin(x^2)</m> is a solution to <m>y' - 12x^2\sin(x^2) = xy''.</m>
			</p>

		</solution>

	</example>

</subsection>