<subsection xmlns:xi="http://www.w3.org/2001/XInclude"><title> Additional Examples </title>

	<example><title> <em>Solution Verification</em> </title>
		<p>
			Is <m>y= 3\sin(x^2)</m> a solution to the DE <m>\quad y' - xy'' = 12x^2\sin(x^2)</m>?
		</p>

		<solution>

			<p>
				<xref ref="solution-verification-step-1" text="title"/>: <m>\quad y' - xy'' - 12x^2\sin(x^2) = 0</m>
			</p>

			<p>
				<xref ref="solution-verification-step-2" text="title"/>. Find <m>y'</m> and <m>y''</m> since they appear in the DE.
				<md>
					<mrow>	y	\amp=  3\sin(x^2)									</mrow>
					<mrow>	y' 	\amp=  3\cos(x^2) \cdot 2x	=	6x\cos(x^2)	</mrow>
					<mrow>	y'' \amp= 6\cos(x^2) - 12x\sin(x^2)	=	6\cos(x^2) - 12x\sin(x^2)	</mrow>
				</md>
			</p>

			<p>
				<xref ref="solution-verification-step-3" text="title"/>. Plug <m>y, y',</m> and <m>y''</m> into the DE and simplify.
				<md>
					<mrow> 												y' - xy'' - 12x^2\sin(x^2) 	\amp= 0									</mrow>
					<mrow> 6x\cos(x^2) - x\left( 6\cos(x^2) - 12x\sin(x^2) \right) - 12x^2\sin(x^2)	\amp= 0									</mrow>
					<mrow> 				\cancel{6x\cos(x^2)} - \cancel{6x\cos(x^2)} - \cancel{12x^2\sin(x^2)} - \cancel{12x^2\sin(x^2)}	\amp= 0									</mrow>
					<mrow> 																		0	\amp= 0	</mrow>
				</md>
				Therefore, <m>y= 3\sin(x^2)</m> is a solution to <m>y' - 12x^2\sin(x^2) = xy''.</m>
			</p>

		</solution>

	</example>

	<example xml:id="verification-with-a-constant"><title> <em>Solution Verification with a Constant</em> </title>
		<p>
			Let <m>C</m> be a constant. Is <m>y = Ce^{2x}</m> a solution to <m>\quad y''' - 4y' = 0</m> ?
		</p>

		<solution>
			
			<p>
				<xref ref="solution-verification-step-2" text="title"/>. Find <m>y'</m> and <m>y'''</m> since they appear in the DE.
				<md>
					<mrow>	y		\amp=  Ce^{2x}	</mrow>
					<mrow>	y'		\amp=  2Ce^{2x}	</mrow>
					<mrow>	y''		\amp=  4Ce^{2x}	</mrow>
					<mrow>	y'''	\amp=  8Ce^{2x}	</mrow>
				</md>
			</p>

			<p>
				<xref ref="solution-verification-step-3" text="title"/>. Plug <m>y, y', y'',</m> and <m>y'''</m> into the DE and simplify.
				<md>
					<mrow> 				y''' - 4y'	\amp= 0 							</mrow>
					<mrow> 	8Ce^{2x} - 4(2Ce^{2x})	\amp= 0 							</mrow>
					<mrow> 		8Ce^{2x} - 8Ce^{2x}	\amp= 0 							</mrow>
					<mrow> 						0	\amp= 0\quad \leftarrow \text{true} </mrow>
				</md>
				Therefore, <m>y = Ce^{2x}</m> is a solution to <m>y''' = 4y'</m>.
			</p>

		</solution>

	</example>
				
	<example><title> <em>Solution Verification with a Constant</em> </title>
		<p>
			Let <m>C_1, C_2</m> be constants. Is <m>y = \frac{1}{2}x^2 + C_1 x + C_2</m> a solution to <m>\quad y'' = 1</m> ?
		</p>
	
		<solution>

			<p>
				<xref ref="solution-verification-step-1" text="title"/>: <m>\quad y'' - 1 = 0</m>
			</p>
	
			<p>
				<xref ref="solution-verification-step-2" text="title"/>. Find <m>y''</m> since it appears in the DE.
				<md>
					<mrow>	y	\amp=  \frac{1}{2}x^2 + C_1 x + C_2									</mrow>
					<mrow>	y' 	\amp=  x + C_1													</mrow>
					<mrow>	y'' \amp=  1														</mrow>
				</md>
			</p>
			<p>
				<xref ref="solution-verification-step-3" text="title"/>. Plug <m>y''</m> into the DE and simplify.
				<md>
					<mrow> 	y'' - 1	\amp= 0	</mrow>
					<mrow> 	1 - 1	\amp= 0	</mrow>
					<mrow> 		0	\amp= 0	</mrow>
				</md>
				Therefore, <m>y = \frac{1}{2}x^2 + C_1 x + C_2</m> is a solution to <m>y'' = 1</m>.
			</p>
	
		</solution>
	
	</example>

	<!-- <example>
		<title> <em>Solution Verification</em> </title>
		<p>
			Is <m>y = x^3 + 2x^2 + Cx + 5</m> a solution to the DE <m>\quad y''' - 6y'' + 12y' - 6y = 0</m>?
		</p>
	
		<solution>
	
			<p>
				<xref ref="solution-verification-step-2" text="title"/>. Find <m>y'</m>, <m>y''</m>, and <m>y'''</m> since they appear in the DE.
				<md>
					<mrow>	y	\amp=  x^3 + 2x^2 + Cx + 5									</mrow>
					<mrow>	y' 	\amp=  3x^2 + 4x + C										</mrow>
					<mrow>	y'' \amp=  6x + 4												</mrow>
					<mrow>	y''' \amp=  6													</mrow>
				</md>
			</p>
	
			<p>
				<xref ref="solution-verification-step-3" text="title"/>. Plug <m>y, y', y'',</m> and <m>y'''</m> into the DE and simplify.
				<md>
					<mrow> 	y''' - 6y'' + 12y' - 6y	\amp=  0											</mrow>
					<mrow> 	6 - 6(6x + 4) + 12(3x^2 + 4x + C) - 6(x^3 + 2x^2 + Cx + 5)	\amp=  0	</mrow>
					<mrow> 	6 - 36x - 24 + 36x^2 + 48x + 12C - 6x^3 - 12x^2 - 6Cx - 30	\amp=  0	</mrow>
					<mrow> 	-6x^3 + 24x^2 + 6C - 36x + 12C - 48	\amp=  0				</mrow>
					<mrow> 	-6x^3 + 24x^2 + 12C - 36x - 48 + 6	\amp=  0					</mrow>
					<mrow> 	-6x^3 + 24x^2 - 36x	+ 12C - 42	\amp=  0						</mrow>
					<mrow> 	-6x^3 + 24x^2 - 36x + 12C - 42	\amp=  0						</mrow>
					<mrow> 	0	\amp=  0														</mrow>
				</md>
				Therefore, <m>y = x^3 + 2x^2 + Cx + 5</m> is a solution to <m>y''' - 6y'' + 12y' - 6y = 0</m>.
			</p>
	
		</solution>
	
	</example>	
	
	<example>
		<title> <em>Solution Verification</em> </title>
		<p>
			Is <m>y = x^3 + Cx + 1</m> a solution to the DE <m>\quad y''' - 4y' + 6y = 6x + 5</m>?
		</p>
	
		<solution>
	
			<p>
				<xref ref="solution-verification-step-1" text="title"/>. Find <m>y'</m> and <m>y'''</m> since they appear in the DE.
				<md>
					<mrow>	y		\amp=  x^3 + Cx + 1	</mrow>
					<mrow>	y'		\amp=  3x^2 + C		</mrow>
					<mrow>	y''		\amp=  6x			</mrow>
					<mrow>	y'''	\amp=  6			</mrow>
				</md>
			</p>
	
			<p>
				<xref ref="solution-verification-step-2" text="title"/>. Plug <m>y, y',</m> and <m>y'''</m> into the DE and simplify.
				<md>
					<mrow> 	y''' - 4y' + 6y	\amp=  6x + 5											</mrow>
					<mrow> 	6 - 4(3x^2 + C) + 6(x^3 + Cx + 1)	\amp=  6x + 5	</mrow>
					<mrow> 	6 - 12x^2 - 4C + 6x^3 + 6Cx + 6	\amp=  6x + 5	</mrow>
					<mrow> 	6x^3 - 12x^2 + 6Cx - 4C + 12	\amp=  6x + 5		</mrow>
					<mrow> 	6x^3 - 12x^2 + 6Cx - 4C + 12 - 6x - 5	\amp=  6x + 5	</mrow>
					<mrow> 	6x^3 - 12x^2 + 6Cx - 6x - 4C + 7	\amp=  6x + 5			</mrow>
					<mrow> 	0	\amp=  0												</mrow>
				</md>
				Therefore, <m>y = x^3 + Cx + 1</m> is a solution to <m>y''' - 4y' + 6y = 6x + 5</m>.
			</p>
	
		</solution>
	
	</example>

	<example>
		<title> <em>Solution Verification</em> </title>
		<p>
			Is <m>y = x^3 + Cx + 1</m> a solution to the DE <m>\quad y''' - 6y' + 6y = 6x + 6</m>?
		</p>
	
		<solution>
	
			<p>
				<xref ref="solution-verification-step-1" text="title"/>. Find <m>y'</m>, <m>y''</m>, and <m>y'''</m> since they appear in the DE.
				<md>
					<mrow>	y	\amp=  x^3 + Cx + 1										</mrow>
					<mrow>	y' 	\amp=  3x^2 + C											</mrow>
					<mrow>	y'' \amp=  6x												</mrow>
					<mrow>	y''' \amp=  6												</mrow>
				</md>
			</p>
	
			<p>
				<xref ref="solution-verification-step-2" text="title"/>. Plug <m>y, y', y'',</m> and <m>y'''</m> into the DE and simplify.
				<md>
					<mrow> 	y''' - 6y' + 6y	\amp=  6x + 6													</mrow>
					<mrow> 	6 - 6(3x^2 + C) + 6(x^3 + Cx + 1)	\amp=  6x + 6			</mrow>
					<mrow> 	6 - 18x^2 - 6C + 6x^3 + 6Cx + 6	\amp=  6x + 6				</mrow>
					<mrow> 	6x^3 - 18x^2 + 6Cx + 12 - 6C	\amp=  6x + 6					</mrow>
					<mrow> 	6x^3 - 18x^2 + 6Cx + 12 - 6C - 6x - 6	\amp=  0				</mrow>
					<mrow> 	6x^3 - 18x^2 + 6Cx - 6x + 6	\amp=  0							</mrow>
					<mrow> 	0	\amp=  0													</mrow>
				</md>
				Therefore, <m>y = x^3 + Cx + 1</m> is a solution to <m>y''' - 6y' + 6y = 6x + 6</m>.
			</p>
	
		</solution>
	
	</example>

	<exercise label="fillin-string-integer"><title>Fill-In, String and Number Answers</title>
		<statement>
			<p>
				Complete the following line of a Python program so that it will declare an integer variable <c>age</c> with an initial value of <c>5</c>.
			</p>
			<p>
				<var /> <c>age = </c> <var /><c>;</c>
			</p>
		</statement>
		<setup>
			<var>
			<condition string="int">
			<feedback>
				<p>
					A variable of type <c>int</c> is appropriate for whole number ages.
				</p>
			</feedback>
			</condition>
			<condition string=".*">
			<feedback>
				<p>
					Remember that Java uses just the first three letters of the word
					<q>integer</q>
					to define an integral type.
				</p>
			</feedback>
			</condition>
			</var>
			<var>
			<condition string="\d">
			<feedback>
				<p>
					An integer variable may be initialized to a value.
				</p>
			</feedback>
			</condition>
			<condition string=".*">
			<feedback>
				<p>
					Use <c>5</c> as the initial value of the variable.
				</p>
			</feedback>
			</condition>
			</var>
		</setup>
	</exercise> -->

	<xi:include href="./p1-c2-s1-2-interactives.ptx" />

</subsection>