<section xmlns:xi="http://www.w3.org/2001/XInclude" xml:id="sec-particular-solutions"><title> Particular Solutions </title>
  
  <introduction>

    <objectives>
      <introduction>
        <p>
        Maybe list some objectives? ...
        </p>
      </introduction>
      <ol>
        <li>objective 1</li>
        <li>objective 2</li>
        <li>objective 3</li>
      </ol>
    </objectives>

    <paragraphs xml:id="algebra-pov"><title> Algebra </title>
      <p>
        When given an algebraic equation such as <m>x^3 - 6x = 4</m>, the solution is all <em>numbers</em>, <m>x</m>, that satisfy the equation. One such solution is <m>x=-2</m>. This can be verified by plugging <m>x=-2</m> into the equation. After simplifying, if the value on the left equals the value on the right, the solution must be valid. When this happens, we say that the solution "satisfies" this equation.
        <sidebyside widths="40% 40%" margin="0%" valign="bottom">
          
          <p>
            <md>
              <mrow>                            x^3 - 6x  \amp = 4 </mrow>
              <mrow> \left(-2\right)^3 - 6\left(-2\right) \amp = 4 </mrow>
              <mrow>                              -8 + 12 \amp = 4 </mrow>
              <mrow>                                    4 \amp = 4 \, \checkmark </mrow>
            </md>  
          </p>
          
          <p>
            The number, <m>x=-2</m>, is a solution since it "satisfies" this equation.
          </p>
          
        </sidebyside>
      </p>

      <p>
        In contrast, when solving a differential equation such as <m>y' - 6y = 10x - 5</m>, we are looking for all <em>functions</em>, <m>y</m>, that satisfy the equation. One solution is <m>y = -5x</m> and we can verify it in the same way.

        <sidebyside widths="50% 30%" valign="bottom">
          
          <p>
            <md>
              <mrow>                                      y' - 2y   \amp = 10x - 5 </mrow>
              <mrow> \left(-5x\right)^{\prime} - 2\left(-5x\right)  \amp = 10x - 5 </mrow>
              <mrow>                                      -5 + 10x  \amp = 10x - 5 </mrow>
              <mrow>                                        10x - 5 \amp = 10x - 5 \, \checkmark </mrow>
            </md>
          </p>
          
          <p>
            The function, <m>y = -5x</m>, is a solution since it "satisfies" this equation.
          </p>
          
        </sidebyside>

      </p>
          
    </paragraphs>

    <paragraphs><title> An Analogy </title>
      <p>
        It is helpful to make an analogy here by thinking about what it means to be a solution to an algebraic equation. Consider (<em> but don't solve!</em>) the following problem and think about the questions that follow.
      </p>

      <p>
        What does it mean when we say <m>x = -1</m> is a solution to the equation below?
        <me> x^5 + 12x^2 +10x = 7x^3 + 24 </me>
      </p>

      <question>
        <title>What does solution mean in this case?</title>

        <p>
          In the context of this equation, a solution would be an <m>x</m>-value that "works" when we substitute it back into the equation (i.e. it satisfies the equation). If we substitute <m>x = -1</m> into each side of the equation, we have
          <md>
            <mrow>\mbox{left hand side of the equation (LHS)}	%\amp= x^5 + 12x^2 +10x,</mrow>
            <mrow>							\amp= (-1)^5 + 12(-1)^2 +10(-1),</mrow>
            <mrow>							\amp= -1 + 12 - 11,</mrow>
            <mrow>							\amp= 0,</mrow>
          </md>
          and
          <md>
            <mrow>\mbox{right hand side of the equation (RHS)}	%\amp= 7x^3 + 24,</mrow>
            <mrow>								\amp= 7(-1)^3 + 24,</mrow>
            <mrow>								\amp= -7 + 24,</mrow>
            <mrow>								\amp= 17.</mrow>
          </md>
        </p>

        <p>
          When we substitute <m>x = -1</m> into the left hand side of the equation we get <m>0</m>, whereas we get <m>17</m> on the right hand side. This means <m>x = -1</m> isn't a solution to the algebraic equation. However, if we try <m>x = -3,</m> we have
          <md>
            <mrow>\mbox{LHS}	%\amp= x^5 + 12x^2 +10x,</mrow>
            <mrow>							\amp= (-3)^5 + 12(-3)^2 +10(-3),</mrow>
            <mrow>							\amp= -243 + 108 - 30,</mrow>
            <mrow>							\amp= -165,</mrow>
          </md>
          and
          <md>
            <mrow>\mbox{RHS}	%\amp= 7x^3 + 24,</mrow>
            <mrow>								\amp= 7(-3)^3 + 24,</mrow>
            <mrow>								\amp= -189 + 24,</mrow>
            <mrow>								\amp= -165.</mrow>
          </md>
        </p>

        <p>
          Since we get the same result when we substitute <m>x = -3</m> in on the left hand and right hand sides of the equation, we can conclude that <m>x = -3</m> is a solution to the algebraic equation.
        </p>

      </question>

      <p>
        Let's take a moment to highlight some important details about how the previous example gives insight into the concept of a solution to a differential equation.
      </p>

      <ul>
        <li>
          Your intuition for algebra should tell you that there is probably more solutions than <m>x = -3</m> to this equation (and you'd be correct). It turns out that differential equations also can have multiple solutions!
        </li>
        <li>
          At no point did we discuss the technique needed to find the solution <m>x = -3</m>. However, this did not stop us from verifying that it was a solution. This fact also transfers to differential equations! Indeed, as you will see in the exercises, given a function, you will be able to verify whether this function is (or is not) a solution to a differential equation.
        </li>
      </ul>

    </paragraphs>

    <p>
      We have just discussed some important ideas that will aid us in understanding what it means to be a solution to an differential equation. You will see that the next two statement are practically identical (except the blue terms).
    </p>

    <ul>
      <li>
        <m>\color{blue}{x}</m> (a <m>\color{blue}{\text{number}}</m>) is a solution to an <m>\color{blue}{\text{algebraic}}</m> equation if we get the same result on the left and right-hand side of the equation after substituting <m>\color{blue}{x}</m> into the entire equation.
      </li>
      <li>
        <m>\color{blue}{y}</m> (a <m>\color{blue}{\text{function}}</m>) is a solution to a <m>\color{blue}{\text{differential}}</m> equation if we get the same result on the left and right-hand side of the equation after substituting <m>\color{blue}{y}</m> into the entire equation.
      </li>
    </ul>
    
    <!--
      <p>
        Recall, <m>\color{blue}{x}</m> (a <m>\color{blue}{\text{number}}</m>) is a solution to an <m>\color{blue}{\text{algebraic}}</m>	equation if:
        <sidebyside widths="90%" margins="auto" valign="middle">
          <p>
            If we get the same result on the left and right-hand side of the equation after plugging <m>\color{blue}{x}</m> into the entire equation, then we say <m>\color{blue}{x}</m> is a solution to the <m>\color{blue}{\text{algebraic}}</m> equation.
          </p>
        </sidebyside>
      </p>
      <p>
        Similarly, <m>\color{blue}{y}</m> (a <m>\color{blue}{\text{function}}</m>) is a solution to an <m>\color{blue}{\text{differential}}</m> equation if:
        <sidebyside widths="90%" margins="auto" valign="middle">
          <p>
            If we get the same result on the left and right-hand side of the equation after plugging <m>\color{blue}{y}</m> into the entire equation, then we say <m>\color{blue}{y}</m> is a solution to the <m>\color{blue}{\text{differential}}</m> equation.
          </p>
        </sidebyside>
      </p>
      -->
      

    <p>
      In all of the previous examples, we verified that one particular function was a solution to the DE, but as previously mentioned, we know that there may be more. It turns out, differential equations generally have infinitely many solutions. We can use <xref ref="example-de-solution-05" /> to illustrate this.
    </p>

    <p>
      In this example, we showed that the function <m>y = c_1e^{-3t} + c_2e^{4t}</m> was a solution <m>y'' - y' - 12y = 0</m>.
    </p>

    <p>
      Notice that we were able to verify the solution, even though the constants, <m>c_1</m> and <m>c_2</m>, were not known. This suggests that you can substitute any values of <m>c_1</m> and <m>c_2</m> into the solution and it will still be a solution to the DE. <em> Try it! </em>
    </p>

    <p>
      Now, since there are infinitely many choices for <m>c_1</m> and <m>c_2</m>,	then, logically, there must be infinitely many solutions to the DE,	<m>y'' - y' - 12y = 0</m>.
    </p>

    <definition xml:id="def-general-solution">
      <statement>
        Given a differential equation, the collection of all solutions of this DE is called the <term>family of solutions</term> of this DE. The form of these solutions is called the <term>general solution</term> of this DE. A single solution from the family of solutions is called a <term>particular solution</term>.
      </statement>
    </definition>

    <remark xml:id="remark-general-solution-01">
      <p>
        A <em>family of solutions</em> can be viewed as the collection of all <em>particular solutions</em>. Conversely, a <em>particular solution</em> can be viewed as a member of the <em>family of solutions</em>.
      </p>
    </remark>

    <p>
      In the context of <xref ref="example-de-solution-05" />, all of the following would be true:
      <ul>
        <li> 	<m>y = c_1e^{-3t} + c_2e^{4t}</m> is the solution to
          <m>y'' - y' - 12y = 0</m>. </li>
        <li> 	<m>y = c_1e^{-3t} + c_2e^{4t}</m> is the <term>general solution</term>
          to the <m>y'' - y' - 12y = 0</m>. </li>
        <li> 	Any solution that has the form: <m>y = c_1e^{-3t} + c_2e^{4t}</m> is in the <term>family of solutions</term> for
          <m>y'' - y' - 12y = 0</m>. </li>
        <li> 	<m>y = -e^{-3t} + 7e^{4t}</m> is a <term>particular solution</term> to
          <m>y'' - y' - 12y = 0 \,\,</m> (<m>c_1 = -1</m>, <m>c_2 = 7</m>).</li>
        <li> 	<m>y = -e^{-3t} + 7e^{4t}</m> is in the <term>family of solutions</term> for <m>y'' - y' - 12y = 0</m> since it has the form:
          <m>y = c_1e^{-3t} + c_2e^{4t}</m> where <m>c_1 = -1</m> and
          <m>c_2 = 7</m>.</li>
      </ul>
    </p>

    <remark xml:id="remark-general-solution-02">
      <p>
        When working on your own problems, remember that the following three statements are referring to the exact same thing.
        <ul>
          <li> Solve the following DE. </li>
          <li> Find the <em>general solution</em> to the following DE. </li>
          <li> Find the <em>family of solutions</em> for the following DE. </li>
        </ul>
      </p>
    </remark>

    <p>
    We spend a lot of time solving equations, but do you even remember what it means to be
    a solution? Let's review what it means to be a solution to an algebraic equation 
    (as in question <xref ref="alg_eqn_soln"/>), and then what it means to be a solution to a differential equation (as in question <xref ref="diff_eqn_soln"/>), and then we'll extend those ideas in questions <xref ref="soln_form1"/> and <xref ref="soln_form2"/>.

    <ol>
      <li>
      <p>
      Verify that <m>x = 3</m> is a solution to the equation 
      
      <men xml:id="alg_eqn_soln">2x^2 + 3 = 7x.</men>
      
      </p>
      
      <p>
      What confirms that <m>x = 3</m> is a solution? 
      <answer>
        the LHS = RHS after substituting <m>x = 3</m> into both sides of the equation.
      </answer>	
      </p>
      
      <p>	
      (<em> Note: Do not rearrange the equation to solve for <m>x</m>. That would be the
      process of finding a solution; you are asked to verify a solution.</em>)
      </p>	
      <p/>
      <solution>
      We substitute <m>x = 3</m> into the left hand side (LHS) of the equation, 
      and then into the right hand side (RHS) of the equation:
      
      <md>
        <mrow>\text{LHS}	\amp= 2x^2 + 3										</mrow>
        <mrow>				\amp= 2(3)^2 + 3									</mrow>
        <mrow>				\amp= 18 + 3										</mrow>
        <mrow>				\amp= 21											</mrow>
        <mrow>				\amp 												</mrow>
        <mrow>\text{RHS}	\amp= 7x											</mrow>
        <mrow>				\amp= 7(3)											</mrow>
        <mrow>				\amp= 21											</mrow>	
      </md>
      
      Since we get the same result when we substitute the solution into the RHS and 
      into the LHS, we have confirmed that <m>x = 3</m> is a solution to the equation.
      </solution>
      <!-- Is this answer necessary?
      <answer>
        Since we get the same result (21) when we substitute the solution into the 
        RHS and into the LHS, we confirm that <m>x = 3</m> is a solution to the equation.
      </answer>
      -->
      
      </li>

      <li>
      <p>
      Verify that <m>y = c_1 \sin x + c_2 \cos x</m> is a solution to the DE 
      
      <men xml:id="diff_eqn_soln">\DS \frac{d^2y}{dx^2} + y = 0.</men>
      
      </p>
      
      <hint>
      Look back at the previous question and think about what it means to be a solution 
      to a DE.
      </hint>
      <solution>
      We need to substitute into the DE. In order to substitute into the left hand side, 
      we need to know the second derivative. So we begin by finding that.
      
      <md>
        <mrow>						y	\amp= c_1 \sin x + c_2 \cos x			</mrow>
        <mrow>	\Rightarrow \quad   y'	\amp= c_1 \cos x - c_2 \sin x			</mrow>
        <mrow>	\Rightarrow \quad   y''	\amp= -c_1 \sin x - c_2 \cos x			</mrow>	
      </md>
        
      Now we can substitute into the DE:
      
      <md>
        <mrow>\text{LHS}\amp= \frac{d^2y}{dx^2} + y								</mrow>
        <mrow>			\amp= \Big[ -c_1 \sin x - c_2 \cos x \Big] 
                      + \Big[ c_1 \sin x + c_2 \cos x \Big]		</mrow>
        <mrow>			\amp= 0													</mrow>
        <mrow>			\amp= \text{RHS}										</mrow>	
      </md>
      
      Since when we substitute in to the DE, we find that the LHS is equal to the RHS, 
      we have verified that <m>y = c_1 \sin x + c_2 \cos x</m> is a solution to the DE
      <m>\DS \frac{d^2y}{dx^2} + y = 0.</m>
      </solution>
      <answer>
        Since we get the same result (0) when we substitute the solution into the RHS 
        and into the LHS, we confirm that <m>y = c_1 \sin x + c_2 \cos x</m> is a
        solution to the DE.
      </answer>
      </li>
      <!-- Do we need this?
      <li xml:id="soln_form1"> 
      <p>
      <em> Assuming the form of the solution of DE.</em> 
                          <!- from Nagle, Saff and Snider ->
      </p>
      </li>
      -->
      <li> 
      <p>
      Consider the DE 
      
      <men xml:id="soln_form1">\DS \frac{d^2 y}{dx^2} + 6 \frac{dy}{dx} + 5y = 0.</men>
      
      </p>
      
      <p>		
      Find all values of <m>m</m> such that <m>y = e^{mx}</m> is a solution to the DE 
      by taking derivatives and substituting into the DE, and then solving for <m>m</m>.
      </p>
        
      <hint>
        <m>e^{mx} \ne 0,</m> no matter the value of <m>x</m> or <m>m.</m> 
        Therefore we might want to factor it out as it won't contribute to our answer.
      </hint>
      <solution>
      First we take derivatives so that we can substitute into the DE.
      
      <md>
        <mrow>						y	\amp= e^{mx}							</mrow>
        <mrow>	\Rightarrow \quad   y'	\amp= me^{mx}							</mrow>
        <mrow>	\Rightarrow \quad   y''	\amp= m^2 e^{mx}						</mrow>	
      </md> 

      Now we can substitute into the DE and solve for <m>m</m>:

      <md>
        <mrow>\frac{d^2 y}{dx^2} 
                + 6 \frac{dy}{dx} + 5y	\amp= 0							</mrow>
        <mrow>\Big[ m^2 e^{mx} \Big] + 6\Big[ m e^{mx} \Big] 
                + 5\Big[ e^{mx} \Big]	\amp= 0							</mrow>
        <mrow>	e^{mx} \Big[ m^2 + 6m + 5 Big]	\amp= 0							</mrow>
        <mrow>				e^{mx} (m+5)(m+1)	\amp= 0							</mrow>	
      </md>
      
      Recall that <m>e^{mx} \ne 0,</m> no matter the value of <m>x</m> or <m>m.</m>
      Thus we have:
      
      <md>
        <mrow>	m+5 = 0 \amp \text{ or } m+1 = 0								</mrow>
        <mrow>	m = -5,	\amp \text{ or } m = -1									</mrow>	
      </md>
      So the two solutions are <m>m = -5, -1.</m>
      </solution>
      <answer>
        <me> m = -5, -1 </me>
      </answer>
      </li>
      <li>
      <p>
      Now that you have (hopefully!) two values for <m>m,</m> choose one of the two values 
      and then verify that <m>y = e^{mx}</m> is a solution for that value of <m>m.</m>
      </p>
      <solution>
      <p>
      The work here is for <m>m = -5,</m> and the work for <m>m = -1</m> is similar.
      </p>
      <p>
      First we take derivatives so that we can substitute into the DE.
      
      <md>
        <mrow>							y	\amp= e^{-5x}						</mrow>
        <mrow>		\Rightarrow \quad   y'	\amp= -5e^{-5x}						</mrow>
        <mrow>		\Rightarrow \quad 	y''	\amp= 25 e^{-5x}					</mrow>	
      </md> 
        
      Now we can substitute into the DE:
      
      <md>
        <mrow>\text{LHS}\amp= \frac{d^2 y}{dx^2} + 6 \frac{dy}{dx} + 5y			</mrow>
        <mrow>			\amp= \Big[ 25e^{-5x} \Big] + 6\Big[ -5e^{-5x} \Big] 
                              + 5\Big[ e^{-5x} \Big]		</mrow>
        <mrow>			\amp= 25e^{-5x} - 30 e^{-5x} + 5e^{-5x}					</mrow>
        <mrow>			\amp= 0													</mrow>
        <mrow>			\amp= \text{RHS}										</mrow>	
      </md>
      
      Hence, we have shown that <m>y = e^{-5x}</m> is a solution to the DE 
      <m>\DS  \frac{d^2 y}{dx^2} + 6 \frac{dy}{dx} + 5y = 0.</m>
      </p>
      </solution>
      <answer>
        Since we get the same result (0) when we substitute the solution into the RHS 
        and into the LHS, we confirm that <m>y = e^{-5x}</m> (or <m>y = e^{-x}</m>) 
        is a solution to the DE.
      </answer>
      </li>
      <li> 
      <!-- Do we need this?
      <p>
      <em> Assuming the form of the solution of DE. </em>
      </p>
      -->
      
      <p>
      Find all values of <m>m</m> such that <m>y = x^m</m> is a solution of the DE 
      
      <men xml:id="soln_form2">\DS 3x^2 \frac{d^2y}{dx^2} = -11x \frac{dy}{dx} + 3y.</men>
      </p>
      <solution>
      <p>
      We proceed as in the previous question. First we take derivatives so that we can substitute into the DE.
      
      <md>
        <mrow>						y	\amp= x^m								</mrow>
        <mrow>	\Rightarrow \quad   y'	\amp= mx^{m-1}							</mrow>
        <mrow>	\Rightarrow \quad   y''	\amp= m(m-1)x^{m-2}						</mrow>	
      </md> 
        
      Now we can substitute into the DE:
      
      <md>
        <mrow>				3x^2 \frac{d^2y}{dx^2}	\amp= 
                      -11x \frac{dy}{dx} + 3y						</mrow>
        <mrow>		3x^2\Big[ m(m-1)x^{m-2} \Big]	\amp= 
                      -11x\Big[ mx^{m-1} \Big] + 3\Big[ x^m \Big]	</mrow>
        <mrow>					3m(m-1)x^2 x^{m-2}	\amp= 
                      -11mx^1\cdot x^{m-1} + 3x^m					</mrow>
        <mrow>				(3m^2 - 3m)x^{2+(m-2)}	\amp= 
                      -11m x^{1 + (m-1)} + 3x^m					</mrow>
        <mrow>					(3m^2 - 3m)x^{m}	\amp= -11m x^{m} + 3x^m		</mrow>
        <mrow>(3m^2 - 3m)x^{m} + 11m x^{m} - 3x^m	\amp= 0						</mrow>
        <mrow>			(3m^2 - 3m + 11m - 3)x^m	\amp= 0						</mrow>
        <mrow>					(3m^2 +8m - 3)x^m	\amp= 0						</mrow>
        <mrow>						(3m -1)(m+3)x^m	\amp= 0						</mrow>	
      </md>
      Note that there is no value of <m>m</m> that can guarantee that <m>x^m</m> is 0.
      Hence we have
        
      <md>
        <mrow>			3m-1 = 0 \amp \quad\text{or}\quad m+3 = 0				</mrow>
        <mrow>	m = \frac{1}{3}, \amp \quad\text{or}\quad m = -3				</mrow>	
      </md>
      So the two solutions are <m>m = -3, \frac{1}{3}.</m>
      </p>
      </solution>
      <answer>
        <me> m = -3, \frac{1}{3} </me>
      </answer>
      </li>
    </ol>
    </p>

  </introduction>

	<xi:include href="./p1-c3-s2-interactives.ptx" />
	<xi:include href="./p1-c3-s2-exercises.ptx" />

</section>