<subsection xml:id="general-solutions-examples"><title> Examples </title>
    
  <p>
    Let's look at a couple of examples to see how this works.
  </p>
  
  <example xml:id="example-de-solution-01">
  
    <p>
      Verify that <m>\DS y = Ce^{x^2} + 3</m>, where <m>C</m> is any constant, is a solution to the DE
      <me>\DS \frac{dy}{dx} = 2xy - 6x.</me>
    </p>
  
    <solution>
  
      <p>
        We'll approach this the same way we approached the algebraic equation in the example above: we will to substitute the function <m>\DS y = Ce^{x^2} + 3</m> in on the left and right hand sides of the equation
  
        <sidebyside widths="45% 55%" margins="auto" valign="top" halign="center">
          <p>
            <md>
              <mrow> \overset{LHS\vphantom{\Big|}}{\frac{dy}{dx}}
                \amp=\frac{d}{dx}\left( Ce^{x^2} + 3 \right)</mrow>
              <mrow> 	\amp= C\frac{d}{dx}\left( e^{x^2} \right) + \frac{d}{dx}\left( 3 \right)</mrow>
              <mrow> 	\amp= C \cdot e^{x^2} \cdot \frac{d}{dx}\left( x^2 \right) + 0</mrow>
              <mrow> 	\amp=  C \cdot e^{x^2} \cdot 2x</mrow>
              <mrow> 	\amp=  2Cxe^{x^2}</mrow>
            </md>
          </p>
          <p>
            <md>
              <mrow> 	\overset{RHS\vphantom{\Big|}}{2xy - 6x}
                \amp= 2x \left( Ce^{x^2} + 3 \right) - 6x</mrow>
              <mrow> 	\amp= 2Cxe^{x^2} + 6x - 6x</mrow>
              <mrow> 	\amp= 2Cxe^{x^2}</mrow>
            </md>
          </p>
        </sidebyside>
  
        Since both the <m>LHS</m> and <m>RHS</m> turn out to be	<m>2Cxe^{x^2}</m>, we have shown that <m>\DS y = Ce^{x^2} + 3</m> satisfies and is, thus, a	solution to	<m>\DS \frac{dy}{dx} = 2xy - 6x.</m>
      </p>
  
    </solution>
  
  </example>
  
  <p>
    Since we used a generic constant <m>C</m>, we have shown that <m>\DS y = Ce^{x^2} + 3</m> is a solution for any value we like for the constant <m>C</m>. In particular,
    <ul>
      <li>for <m>C=-41, \quad y = -41e^{x^2} + 3 \quad</m> is a solution.</li>
      <li>for <m>C=199, \quad y = 199e^{x^2} + 3 \quad</m> is a solution.</li>
      <li>for <m>C=0, \quad y = 3 \quad</m> is a solution.</li>
    </ul>
    Since there is no limit to what <m>C</m> we can choose, this DE must have an infinite number of solutions. In the next section, we will describe this idea further.
  </p>
  
  <example xml:id="example-de-solution-02">
  
    <p>
      Verify that <m>\DS y = 3\sin(x^2)</m> is a solution to the DE
      <me>y' - 12x^2\sin(x^2) = xy''</me>.
    </p>
  
    <solution>
  
      <p>
        First, let's compute <m>y'</m> and <m>y''</m> since we will need to plug them into the DE.
        <md>
          <mrow>y'	\amp= \frac{d}{dx}\left( 3\sin(x^2) \right)</mrow>
          <mrow>		\amp= 3\cos(x^2) \cdot \frac{d}{dx}\left( x^2\right) \hspace{0.2cm}\mbox{(using the chain rule)}</mrow>
          <mrow>		\amp= 3\cos(x^2) \cdot 2x</mrow>
          <mrow>		\amp= 6x\cos(x^2)</mrow>
          <mrow>		\amp</mrow>
          <mrow>y''	\amp= 6x \cdot \frac{d}{dx}\left( \cos(x^2) \right) + \frac{d}{dx}\left( 6x \right)\cdot \cos(x^2) \hspace{0.2cm} \mbox{(using the product rule)}</mrow>
          <mrow>		\amp= -12x^2\sin(x^2) + 6\cos(x^2)</mrow>
        </md>
      </p>
  
      <p>
        With these in hand, we can substitute into the left and right hand sides of the equation, as follows.
        <md>
          <mrow>\mbox{LHS} 	\amp= y' - 12x^2\sin(x^2) </mrow>
          <mrow>						\amp= 6x\cos(x^2) - 12x^2\sin(x^2)</mrow>
          <mrow> 						\amp</mrow>
          <mrow>\mbox{RHS} 	\amp= xy'' 	</mrow>
          <mrow>						\amp= x\left( -12x^2\sin(x^2) + 6\cos(x^2) \right)</mrow>
          <mrow> 						\amp= -12x^3\sin(x^2) + 6x\cos(x^2)</mrow>
        </md>
      </p>
  
      <p>
        The resulting expressions left hand side and the right hand side are similar, but they are not the same. Hence,
        <m>y = 3\sin(x^2)</m> is <term> not a solution </term> to <m>y' - 12x^2\sin(x^2) = xy''</m>.
      </p>
  
    </solution>
  
  </example>
  
  <example xml:id="example-de-solution-03">
  
    <p>
      Determine if <m>y= 2e^{-3t}</m> is a solution to the DE <m>y'' - y' - 12y = 0</m>.
    </p>
  
    <solution>
  
      <p>
        As in the previous example, we need to substitute <m>y, y',</m> and <m>y''</m> into the DE.
        <md>
          <mrow>	y	\amp= 2e^{-3t} 	\hspace{-0.4cm}\amp\Rightarrow \hspace{0.1cm}
            y'	\amp= -6e^{-3t}	\hspace{-0.4cm}\amp\Rightarrow \hspace{0.1cm}
            y''	\amp= 18e^{-3t}
          </mrow>
        </md>
      </p>
  
      <p>
        Now let's substitute these expressions into the DE.
        <md>
          <mrow>LHS	\amp= y'' - y' - 12y									</mrow>
          <mrow>		\amp= \left(18e^{-3t}\right) - \left( -6e^{-3t} \right)
            - 12\left( 2e^{-3t} \right)		</mrow>
          <mrow>		\amp= 18e^{-3t} + 6e^{-3t} - 24e^{-3t}					</mrow>
          <mrow>		\amp= 0													</mrow>
          <mrow>		\amp= RHS												</mrow>
        </md>
        So, yes, <m>y= 2e^{-3t}</m> is a solution to <m>y'' - y' - 12y = 0.</m>
      </p>
  
    </solution>
  
  </example>
  
  <example xml:id="example-de-solution-04">
  
    <p>
      Determine if <m>y = e^{4t}</m> is a solution to the DE <m>y'' - y' - 12y = 0</m>.
    </p>
  
    <solution>
  
      <p>
        <md>
          <mrow>	y	\amp= e^{4t} 	\hspace{-0.4cm}\amp\Rightarrow \hspace{0.1cm}
            y'	\amp= 4e^{4t}	\hspace{-0.4cm}\amp\Rightarrow \hspace{0.1cm}
            y''	\amp= 16e^{4t}
          </mrow>
        </md>
  
        <md>
          <mrow>LHS	\amp= y'' - y' - 12y									</mrow>
          <mrow>		\amp= \left(16e^{4t}\right) - \left( 4e^{4t} \right)
            - 12\left( e^{4t} \right)			</mrow>
          <mrow>		\amp= 16e^{4t} - 4e^{4t} - 12e^{4t}						</mrow>
          <mrow>		\amp= 0													</mrow>
          <mrow>		\amp= RHS												</mrow>
        </md>
        So, yes, <m>y = e^{4t}</m> is a solution to <m>y'' - y' - 12y = 0.</m>
      </p>
  
    </solution>
  
  </example>
  
  <example xml:id="example-de-solution-05">
  
    <p>
      Determine if <m>y = c_1e^{-3t} + c_2e^{4t}</m> is a solution to the DE
      <m>y'' - y' - 12y = 0</m> where <m>c_1</m> and <m>c_2</m> are constants.
    </p>
  
    <solution>
      <p>
        Find <m>y, y', \text{ and } y''</m>.
        <md>
          <mrow>y		\amp= c_1e^{-3t} + c_2e^{4t} \hspace{-0.4cm}
            \amp\Rightarrow\hspace{0.1cm}
            y'	\amp= -3c_1e^{-3t} + 4c_2e^{4t} \hspace{-0.4cm}
            \amp\Rightarrow\hspace{0.1cm}
            y''	\amp= 9c_1e^{-3t} + 16c_2e^{4t}
          </mrow>
        </md>
      </p>
  
      <p>
        and substitute
        <md>
          <mrow>LHS	\amp= y'' - y' - 12y										</mrow>
          <mrow>		\amp= \left(9c_1e^{-3t} + 16c_2e^{4t}\right)
            - \left( -3c_1e^{-3t} + 4c_2e^{4t} \right)
            - 12\left( c_1e^{-3t} + c_2e^{4t} \right)				</mrow>
          <mrow>		\amp= 9c_1e^{-3t} + 16c_2e^{4t} + 3c_1e^{-3t}
            - 4c_2e^{4t} - 12c_1e^{-3t} - 12c_2e^{4t}			</mrow>
          <mrow>		\amp= \left( 9c_1e^{-3t} + 3c_1e^{-3t} - 12c_1e^{-3t} \right)
            + \left( 16c_2e^{4t} - 4c_2e^{4t} - 12c_2e^{4t} \right)	</mrow>
          <mrow>		\amp = 0													</mrow>
          <mrow>		\amp= RHS													</mrow>
        </md>
        Which shows that <m>y = c_1e^{-3t} + c_2e^{4t}</m> is a solution to <m>y'' - y' - 12y = 0.</m>
      </p>
  
    </solution>
  
  </example>
  
  <example xml:id="example-de-solution-06">
  
    <statement>
        <p>
            Verify that <m>y = Ce^{-5x^2} + \frac{3}{5}</m> is a solution to the DE
            <me>\frac{dy}{dx} = \big( 2x \big) \big( 3 - 5y \big)</me>
        </p>
    </statement>
  
    <solution>
        <p>
            Working out the left and right hand sides of this DE, we have:
  
            <sidebyside widths="45% 55%" margins="auto" valign="top" halign="center">
            <p>
                <md>
                    <mrow> LHS: </mrow>
                    <mrow> \frac{dy}{dx}
                            \amp=\frac{d}{dx}\left( Ce^{-5x^2} + \frac{3}{5} \right)</mrow>
                    <mrow> 	\amp= Ce^{-5x^2} \cdot \frac{d}{dx}(-5x^2) + 0</mrow>
                    <mrow> 	\amp= Ce^{-5x^2} \cdot -10x</mrow>
                    <mrow> 	\amp= -10Cxe^{-5x^2}</mrow>
                </md>
            </p>
            <p>
                <md>
                    <mrow> RHS: </mrow>
                    <mrow> 	\big(2x\big)\amp\big(3 - 5y\big)</mrow>
                    <mrow> 	\amp= 2x \left[3 - 5\left(Ce^{-5x^2} + \frac{3}{5}\right) \right]</mrow>
                    <mrow> 	\amp= 2x \left[ 3 - 5Ce^{-5x^2} - 3 \right]</mrow>
                    <mrow> 	\amp= 2x \left[-5Ce^{-5x^2}\right]</mrow>
                    <mrow> 	\amp= -10Cxe^{-5x^2}</mrow>
                </md>
            </p>
            </sidebyside>
        </p>
  
        <p>
            Since <m>LHS = RHS</m>, we have verified that
            <m>y = Ce^{-5x^2} + \frac{3}{5}</m> is a solution to
            <me>\frac{dy}{dx} = \big( 2x \big) \big( 3 - 5y \big)</me>
        </p>
    </solution>
  
  </example>
  
  <p>
    Edit Notes:
    <ul>
      <li> perhaps add concluding thought to the progression of examples that showed linear combinations of solutions were also a solution in this particular case? Or just wait until the next subsection? </li>
    </ul>
  </p>
  
    <exercises>
      <title> Now you Try </title>
      
          <ul marker="">
            <li>
              <exercise><title> True or False. An equation that contains an "=" sign and at least one derivative is called a differential equation </title>
                <statement correct="yes"/>
                <feedback>
                  A diifferential equation requires both an "=" sign and a derivative.
                </feedback>
              </exercise>
            </li>
      
            <li>
              <p>
                <exercise><title> Fill-In the blank </title>
                  <statement>
                    <ul>
                      <li>When you solve a differential equation, you are finding all <var width="10"/> that satisfies the equation.</li>
                    </ul>
                  </statement>
                  <setup>
                    
                    <var case="insensitive">
            
                      <condition string="functions?"> <feedback> Good Work! </feedback> </condition>
                      
                      <condition string="variables?">
                        <feedback>
                          Yes, variables could be considered a correct answer, but we were looking for <term>functions</term>
                        </feedback>
                      </condition>
                      
                      <condition string=".*">
                        <feedback>
                          <p>
                            Incorrect. Check out the second paragraph of <xref ref="algebra-pov" text="title"/>
                          </p>
                        </feedback>
                      </condition>
                
                      </var>
                  </setup>
                </exercise>
              </p>
            </li>
      
          </ul>
      
      </exercises>
    
  </subsection>